composition/map_gset.fst
@@ -1,0 +1,601 @@
+module Map_gset
+open FStar.List.Tot
+
+open Library
+module C = Gset
+
+type op = (nat (*key*) * C.op)
+
+val get_key : op1:(nat * op) -> Tot (k:nat {exists id v. op1 = (id, (k, C.Add v))})
+let get_key (id, (k, C.Add v)) = k
+
+val get_set : op1:(nat * op) -> Tot (s:C.op {exists id k. op1 = (id, (k, s))})
+let get_set (id, (k, s)) = s
+
+val get_val : op1:(nat * op) -> Tot (v:nat {exists id k. op1 = (id, (k, C.Add v))})
+let get_val (id, (k, C.Add v)) = v
+
+val get_key_s : s:(nat * C.s) -> Tot (s1:nat {(exists c. s = (s1,c))})
+let get_key_s (k, _) = k
+
+val mem_key_s : ele1:nat
+             -> l:list (nat * C.s)
+             -> Tot (b:bool {b=true <==> (exists c. mem (ele1,c) l) /\ (exists e. mem e l /\ get_key_s e = ele1)})
+let rec mem_key_s ele1 l =
+  match l with
+  |[] -> false
+  |x::xs -> get_key_s x = ele1 || mem_key_s ele1 xs
+
+val unique_key : list (nat * C.s) -> bool
+let rec unique_key l =
+  match l with
+  |[] -> true
+  |(ele,_)::xs -> not (mem_key_s ele xs) && unique_key xs
+
+val get_val_s1 : s:(nat * C.s) -> Tot (c:C.s {(exists i. s = (i,c))})
+let get_val_s1 (_, c) = c
+
+type s = l:list (nat * C.s) {unique_key l}
+
+val get_val_s : i:nat -> s1:s -> Tot (c:C.s {(mem_key_s i s1 ==> mem (i,c) s1 /\ (exists e. mem e s1 ==> e = (i,c))) /\ 
+                                              (not (mem_key_s i s1) ==> c = [])})
+let rec get_val_s i s1 =
+  match s1 with
+  |[] -> []
+  |x::xs -> if get_key_s x = i then (get_val_s1 x) else get_val_s i xs
+
+val lemma2 : s1:s 
+           -> Lemma (requires true)
+                   (ensures (forall e. mem e s1 ==> (get_val_s (get_key_s e) s1 = get_val_s1 e)) /\
+                            (forall e. mem e s1 ==> C.unique_s (get_val_s (get_key_s e) s1)))
+                [SMTPat (unique_key s1)]
+#set-options "--z3rlimit 10000000"
+let rec lemma2  s1 = 
+      match s1 with
+      |[] -> ()
+      |x::xs -> lemma2 xs 
+
+val mem_op : ele1:op
+           -> l:list (nat * op)
+           -> Tot (b:bool {b=true <==> (exists id. mem (id, ele1) l) })
+let rec mem_op ele2 l =
+  match l with
+  |[] -> false
+  |(_, ele1)::xs -> ele1 = ele2 || mem_op ele2 xs
+
+val mem_key : i:nat -> l:list (nat * op) -> Tot (b:bool {b=true <==> (exists id op. mem (id, (i, op)) l)})
+let rec mem_key ele2 l =
+    match l with
+    |[] -> false
+    |(_, (ele1, _))::xs -> ele1 = ele2 || mem_key ele2 xs
+
+val filter_uni : #op:eqtype 
+               -> f:((nat * op) -> bool)
+               -> l:list (nat * op) 
+               -> Lemma (requires (unique l ))
+                       (ensures (unique (filter f l)))
+                       [SMTPat (filter f l)]
+let rec filter_uni #op f l =
+  match l with
+  |[] -> ()
+  |x::xs -> filter_uni f xs
+
+val project_op : o1:(nat * op)
+               -> Tot (o2:(nat * C.op) {o2 = (get_id o1, get_set o1)})
+let project_op op =
+    match op with
+    |(id, (k, set)) -> (id, set)
+
+val project1 : i:nat
+             -> l:ae op
+             -> Pure (list (nat * C.op))
+                    (requires true)
+                    (ensures (fun r -> (forall id. member id r <==> member id l.l /\ 
+                                    get_op (get_eve id l.l) = (i, (C.Add (get_val (get_eve id l.l))))) /\
+                                  (forall id. member id r <==> (member id l.l /\ get_key (get_eve id l.l) = i)) /\ unique r /\
+                (forall e. mem e r <==> (mem ((get_id e), (i, C.Add (C.get_ele e))) l.l)) /\
+                (forall e. mem e l.l /\ get_key e = i ==> mem (project_op e) r)))
+            (decreases List.Tot.length l.l)
+
+#set-options "--z3rlimit 10000000"
+let rec project1 i l =
+  match l.l with
+  |[] -> []
+  |x::xs -> if (get_key x = i) then (project_op x)::project1 i (A l.vis xs) else (project1 i (A l.vis xs))
+
+val project : i:nat
+            -> l:ae op
+            -> Pure (ae C.op)
+                   (requires true)
+                   (ensures (fun r -> (forall id. member id r.l <==> member id l.l /\ 
+                                   get_op (get_eve id l.l) = (i, (C.Add (get_val (get_eve id l.l))))) /\
+              (forall id. member id r.l <==> (member id l.l /\ get_key (get_eve id l.l) = i)) /\ unique r.l /\
+                 (forall e. mem e r.l <==> (mem ((get_id e), (i, C.Add (C.get_ele e))) l.l)) /\
+                 (forall e. mem e l.l /\ get_key e = i ==> mem (project_op e) r.l) /\
+                 (forall e e1. (get_id e <> get_id e1 /\ mem (get_id e, (i, C.Add (C.get_ele e))) l.l /\ 
+              mem (get_id e1, (i, C.Add (C.get_ele e1))) l.l /\
+                  l.vis (get_id e, (i, C.Add (C.get_ele e))) (get_id e1, (i, C.Add (C.get_ele e1)))) <==> 
+            (get_id e <> get_id e1 /\ mem e r.l /\ mem e1 r.l /\ r.vis e e1))))
+               (decreases length l.l)
+
+#set-options "--z3rlimit 10000000"
+let project i l =
+              (A (fun o o1 -> (mem (get_id o, (i, C.Add (C.get_ele o))) l.l && mem (get_id o1, (i, C.Add (C.get_ele o1))) l.l &&  get_id o <> get_id o1 && l.vis (get_id o, (i, C.Add (C.get_ele o))) (get_id o1, (i, C.Add (C.get_ele o1))))) (project1 i l))
+
+val app_op : st:s -> op1:(nat * op)
+           -> Pure s 
+             (requires true)
+             (ensures (fun r -> (forall ch. mem_key_s ch r <==> mem_key_s ch st \/ ch = get_key op1) /\
+                             (forall e. mem e (get_val_s (get_key op1) r) <==> 
+                                   mem e (get_val_s (get_key op1) st) \/ e = (get_val op1)) /\
+                             (forall ch. mem_key_s ch st /\ ch <> (get_key op1) ==> 
+                                    (forall e. mem e (get_val_s ch st) <==> mem e (get_val_s ch r)))))
+
+#set-options "--z3rlimit 10000000"
+let rec app_op st op1 =
+  match st with
+  |[] -> [(get_key op1, [get_val op1])]
+  |(ch, x)::xs -> if ch = get_key op1 then (ch, (C.app_op x (project_op op1)))::xs
+                     else (ch, x)::app_op xs op1
+
+instance gmap : datatype s op = {
+  Library.app_op = app_op
+}
+
+#set-options "--query_stats"
+val sim : tr:ae op
+        -> s1:s
+        -> Tot (b:bool {(b = true) <==> (forall ch. mem_key_s ch s1 <==> mem_key ch tr.l) /\
+                                     (forall ch. mem_key_s ch s1 ==> C.sim (project ch tr) (get_val_s ch s1)) /\
+                                     (forall e. mem e tr.l ==> (exists e1. mem e1 s1 /\ get_key e = get_key_s e1 /\
+                                           mem (get_val e) (get_val_s1 e1)))})
+
+#set-options "--z3rlimit 10000000"
+let sim tr s1 = 
+  forallb (fun e -> mem_key (get_key_s e) tr.l) s1 &&
+  forallb (fun e -> mem_key_s (get_key e) s1) tr.l &&
+  forallb (fun e -> C.sim (project (get_key_s e) tr) (get_val_s (get_key_s e) s1)) s1 &&
+  forallb (fun e -> (existsb (fun e1 -> get_key e = get_key_s e1 && mem (get_val e) (get_val_s1 e1)) s1)) tr.l
+
+val lemma4 : tr:ae op -> s1:s
+           -> Lemma (requires sim tr s1)
+                   (ensures (forall i. (C.sim (project i tr) (get_val_s i s1))))
+                      [SMTPat (sim tr s1)]
+let lemma4 tr s1 = ()
+
+val convergence1 : tr:ae op
+                 -> a:s
+                 -> b:s
+                 -> Lemma (requires (sim tr a /\ sim tr b))
+                         (ensures (forall e. mem_key_s e a <==> mem_key_s e b))
+#set-options "--z3rlimit 100000000"
+let convergence1 tr a b = ()
+
+val unique_keys : list nat -> Tot bool
+      let rec unique_keys l =
+      match l with
+      |[] -> true
+      |x::xs -> not (mem x xs) && unique_keys xs
+
+val get_lst : m:s -> Pure (list nat)
+                           (requires true)
+                           (ensures (fun r -> (forall i. mem i r <==> mem_key_s i m) /\ unique_keys r))
+let rec get_lst m =
+          match m with
+          |[] -> []
+          |(i,x)::xs -> i::get_lst xs
+
+val convergence : tr:ae op
+                -> a:s
+                -> b:s
+                -> Lemma (requires (sim tr a /\ sim tr b))
+                        (ensures (forall ch. mem_key_s ch a <==> mem_key_s ch b) /\
+                                 (forall ch. mem_key_s ch a /\ mem_key_s ch b ==>
+                                    (forall e. mem e (get_val_s ch a) <==> mem e (get_val_s ch b))))
+
+#set-options "--z3rlimit 10000000"
+let convergence tr a b =
+  convergence1 tr a b
+
+val lem_oper : tr:ae op 
+             -> op:(nat * op)
+             -> Lemma (requires (not (member (get_id op) tr.l)))
+                     (ensures (forall e. mem e (project (get_key op) (append tr op)).l <==> 
+                                    mem e (append (project (get_key op) tr) (project_op op)).l) /\
+               (forall e e1. mem e (project (get_key op) (append tr op)).l /\
+                        mem e1 (project (get_key op) (append tr op)).l /\ (get_id e <> get_id e1) /\
+                        (project (get_key op) (append tr op)).vis e e1  <==> 
+                        mem e (append (project (get_key op) tr) (project_op op)).l /\
+                    mem e1 (append (project (get_key op) tr) (project_op op)).l /\ get_id e <> get_id e1 /\
+                        (append (project (get_key op) tr) (project_op op)).vis e e1) /\
+         (forall i. i <> (get_key op) ==> (forall e. mem e (project i (append tr op)).l <==> mem e (project i tr).l) /\
+         (forall e e1. mem e (project i (append tr op)).l /\ mem e1 (project i (append tr op)).l /\ get_id e <> get_id e1 /\
+                    (project i (append tr op)).vis e e1 <==> 
+        mem e (project i tr).l /\ mem e1 (project i tr).l /\ get_id e <> get_id e1 /\ (project i tr).vis e e1)))
+
+#set-options "--z3rlimit 10000000"
+let lem_oper tr op = ()
+
+val prop_oper : tr:ae op
+              -> st:s
+              -> op:(nat * op) 
+              -> Lemma (requires (sim tr st) /\ (not (member (get_id op) tr.l)))
+                      (ensures (sim (append tr op) (app_op st op)))
+
+#set-options "--z3rlimit 10000000"
+let prop_oper tr st op = 
+  lem_oper tr op;
+  assert (forall ch. mem_key_s ch (app_op st op) <==> mem_key ch (append tr op).l); 
+  C.prop_oper (project (get_key op) tr) (get_val_s (get_key op) st) (project_op op); 
+  assert (C.sim (project (get_key op) (append tr op)) (get_val_s (get_key op) (app_op st op)));
+  assert (forall e. mem e (append tr op).l ==> (exists e1. mem e1 (app_op st op) /\ get_key e = get_key_s e1 /\
+                                            mem (get_val e) (get_val_s1 e1)));
+  ()
+(*494309 ms*)
+
+val get_key_lst : l:s -> a:s -> b:s
+               -> Pure (list nat)
+                   (requires (forall i. mem_key_s i l ==> mem_key_s i a /\ mem_key_s i b))
+                   (ensures (fun r -> (forall i. mem i r <==> mem_key_s i a \/ mem_key_s i b) /\ unique_keys r))
+                   (decreases %[l;a;b])
+
+let rec get_key_lst l a b =
+  match l,a,b with
+  |[],[],[] -> []
+  |x::xs,_,_ -> get_key_lst xs a b
+  |[],x::xs,_ -> if (mem_key_s (get_key_s x) b) then get_key_lst [] xs b else (get_key_s x)::(get_key_lst [] xs b)
+  |[],[],x::xs -> (get_key_s x)::(get_key_lst [] [] xs)
+
+val merge1 : l:s
+           -> a:s
+           -> b:s
+           -> lst:list nat 
+           -> Pure s
+            (requires (forall e. mem_key_s e l ==> mem_key_s e a /\ mem_key_s e b) /\ unique_keys lst /\
+                      (forall ch. mem ch lst ==> (forall e. mem e (get_val_s ch l) ==>
+                                        mem e (get_val_s ch a) /\ mem e (get_val_s ch b))))
+               (ensures (fun r -> (forall ch. mem_key_s ch r <==> mem ch lst) /\
+                        (forall ch. mem ch lst ==> (get_val_s ch r) =
+                                   (C.merge1 (get_val_s ch l) (get_val_s ch a) (get_val_s ch b))) /\
+                        (forall ch. mem ch lst ==> (forall e. mem e (get_val_s ch r) <==>
+                                     mem e (C.merge1 (get_val_s ch l) (get_val_s ch a) (get_val_s ch b))))))
+             (decreases lst)
+
+#set-options "--z3rlimit 10000000" 
+let rec merge1 l a b lst =
+  match lst with
+  |[] -> []
+  |x::xs -> (x, C.merge1 (get_val_s x l) (get_val_s x a) (get_val_s x b))::merge1 l a b xs
+
+val lem_merge1 : ltr:ae op
+            -> l:s
+            -> atr:ae op
+            -> a:s
+            -> btr:ae op
+            -> b:s
+            -> lst:list nat
+            -> Lemma (requires (forall e. mem e ltr.l ==> not (member (get_id e) atr.l)) /\
+                                  (forall e. mem e atr.l ==> not (member (get_id e) btr.l)) /\
+                                  (forall e. mem e ltr.l ==> not (member (get_id e) btr.l)) /\
+                                  (sim ltr l /\ sim (union ltr atr) a /\ sim (union ltr btr) b) /\
+                                  (forall ch. mem ch lst <==> mem_key_s ch a \/ mem_key_s ch b) /\ unique_keys lst)
+                    (ensures (forall i. mem_key_s i l ==> mem_key_s i a /\ mem_key_s i b) /\
+                             (forall ch. mem ch lst ==> (forall e. mem e (get_val_s ch l) ==>
+                                           mem e (get_val_s ch a) /\ mem e (get_val_s ch b))))
+
+#set-options "--z3rlimit 10000000"
+let lem_merge1 ltr l atr a btr b lst = ()
+
+val merge : ltr:ae op
+          -> l:s
+          -> atr:ae op
+          -> a:s
+          -> btr:ae op
+          -> b:s
+          -> Pure s (requires (forall e. mem e ltr.l ==> not (member (get_id e) atr.l)) /\
+                               (forall e. mem e atr.l ==> not (member (get_id e) btr.l)) /\
+                               (forall e. mem e ltr.l ==> not (member (get_id e) btr.l)) /\
+                               (sim ltr l /\ sim (union ltr atr) a /\ sim (union ltr btr) b))
+                 (ensures (fun r -> (forall i. mem_key_s i l ==> mem_key_s i a /\ mem_key_s i b) /\
+                                 (forall i. mem_key_s i r <==> mem_key_s i a \/ mem_key_s i b) /\
+                 (forall ch. mem_key_s ch r ==> 
+                 (forall e. mem e (get_val_s ch l) ==> mem e (get_val_s ch a) /\ mem e (get_val_s ch b))) /\
+                               (forall ch. mem_key_s ch r ==> (get_val_s ch r) =
+                               (C.merge1 (get_val_s ch l) (get_val_s ch a) (get_val_s ch b))) /\
+                             (forall ch. mem_key_s ch r ==> (forall e. mem e (get_val_s ch r) <==>
+                                        mem e (C.merge1 (get_val_s ch l) (get_val_s ch a) (get_val_s ch b))))))
+
+#set-options "--z3rlimit 10000000"
+let merge ltr l atr a btr b =
+  assert (forall i. mem_key_s i l ==> mem_key_s i a /\ mem_key_s i b);
+  let keys = get_key_lst l a b in
+  assert (forall i. mem i keys <==> mem_key_s i a \/ mem_key_s i b);
+  lem_merge1 ltr l atr a btr b keys;
+  let r = merge1 l a b keys in
+  r
+
+val remove_op1 : tr:ae C.op 
+               -> x:(nat * C.op) 
+               -> Pure (list (nat * C.op))
+                      (requires (mem x tr.l))
+                      (ensures (fun r -> (forall e. mem e r <==> mem e tr.l /\ e <> x) /\ unique r /\ 
+                                      (List.Tot.length r = List.Tot.length tr.l - 1)))
+                 (decreases tr.l)
+
+let rec remove_op1 tr x =
+  match tr.l with
+  |x1::xs -> if x = x1 then xs else x1::remove_op1 (A tr.vis xs) x
+
+val remove_op : tr:ae C.op 
+              -> x:(nat * C.op) 
+              -> Pure (ae C.op)
+                     (requires (mem x tr.l))
+                     (ensures (fun r -> (forall e. mem e r.l <==> mem e tr.l /\ e <> x) /\ unique r.l /\
+                     (forall e e1. mem e tr.l /\ mem e1 tr.l /\ get_id e <> get_id e1 /\ e <> x /\ e1 <> x /\ tr.vis e e1 <==>
+                    mem e (remove_op1 tr x) /\ mem e1 (remove_op1 tr x) /\ get_id e <> get_id e1 /\ tr.vis e e1) /\
+                                (List.Tot.length r.l = List.Tot.length tr.l - 1)))
+                (decreases tr.l)
+let remove_op  tr x =
+    (A (fun o o1 -> mem o (remove_op1 tr x) && mem o1 (remove_op1 tr x) && get_id o <> get_id o1 && tr.vis o o1) (remove_op1 tr x))
+
+val lemma6 : l:ae op 
+           -> a:ae op 
+           -> Lemma (requires (forall e. mem e l.l ==> not (member (get_id e) a.l)))
+                   (ensures (forall e. mem_op e (union1 l a) <==> mem_op e l.l \/ mem_op e a.l))
+                                 (decreases %[l.l;a.l])
+
+#set-options "--z3rlimit 10000000"
+let rec lemma6 l a = 
+  match l,a with
+  |(A _ []), (A _ []) -> ()
+  |(A _ (x::xs)), _ -> lemma6 (A l.vis xs) a
+  |(A _ []), (A _ (x::xs)) -> lemma6 l (A a.vis xs)
+
+val lemma61 : l:ae op
+            -> a:ae op
+            -> b:ae op
+                 -> Lemma (requires (forall e. mem e l.l ==> not (member (get_id e) a.l)) /\
+                                   (forall e. mem e a.l ==> not (member (get_id e) b.l)) /\
+                                   (forall e. mem e l.l ==> not (member (get_id e) b.l)))
+                         (ensures (forall e. mem_op e (absmerge1 l a b) <==> 
+                                        mem_op e l.l \/ mem_op e a.l \/ mem_op e b.l))
+                                        (decreases %[l.l;a.l;b.l])
+
+#set-options "--z3rlimit 10000000"
+let rec lemma61 l a b = 
+    match l,a,b with
+    |(A _ []), (A _ []), (A _ []) -> ()
+    |(A _ (x::xs)), _, _ -> lemma61 (A l.vis xs) a b
+    |(A _ []), (A _ (x::xs)), _ -> lemma61 l (A a.vis xs) b
+    |(A _ []), (A _ []), (A _ (x::xs)) -> lemma61 l a (A b.vis xs)
+
+val remove_ele1 : ele:nat 
+               -> l:(ae C.op) 
+               -> Tot (l1:list (nat * C.op) {(forall e. mem e l1 <==> mem e l.l /\ C.get_ele e <> ele) /\ unique l1})
+               (decreases l.l)
+
+let rec remove_ele1 k l =
+  match l.l with
+  |[] -> []
+  |(id, (C.Add k1))::xs -> if k = k1 then remove_ele1 k (A l.vis xs) else (id, (C.Add k1))::remove_ele1 k (A l.vis xs)
+
+val remove_ele : ele:nat 
+               -> l:(ae C.op) 
+               -> Tot (l1:(ae C.op) {(forall e. mem e l1.l <==> mem e l.l /\ C.get_ele e <> ele) /\
+                                   (forall e e1. mem e l.l /\ mem e1 l.l /\ C.get_ele e <> ele /\ C.get_ele e1 <> ele /\
+                                   get_id e <> get_id e1 /\ l.vis e e1 <==>
+                 mem e (remove_ele1 ele l) /\ mem e1 (remove_ele1 ele l) /\ get_id e <> get_id e1 /\ l1.vis e e1)})
+                  (decreases l.l)
+let remove_ele x tr =
+  (A (fun o o1 -> mem o (remove_ele1 x tr) && mem o1 (remove_ele1 x tr) && get_id o <> get_id o1 && tr.vis o o1) (remove_ele1 x tr))
+
+val remove_st : ele:nat 
+              -> s1:C.s {mem ele s1}
+              -> Tot (s2:C.s {forall e. mem e s2 <==> mem e s1 /\ e <> ele})
+let rec remove_st ele s1 =
+  match s1 with
+  |x::xs -> if x = ele then xs else x::remove_st ele xs
+
+val lemma7 : tr:ae C.op -> s1:C.s -> tr1:ae C.op
+           -> Lemma (requires C.sim tr s1 /\ (forall e. mem e tr1.l <==> mem e tr.l) /\
+                             (forall e e1. mem e tr1.l /\ mem e1 tr1.l /\ get_id e <> get_id e1 /\ tr1.vis e e1 <==>
+                                      mem e tr.l /\ mem e1 tr.l /\ get_id e <> get_id e1 /\ tr.vis e e1))
+                   (ensures (C.sim tr1 s1))
+                     (decreases %[tr.l;s1;tr1.l])
+
+#set-options "--z3rlimit 10000000"
+let rec lemma7 tr s1 tr1 = 
+  match tr.l, tr1.l with
+  |[], [] -> ()
+  |(id, (C.Add v))::xs, _ -> 
+               if (C.mem_ele v xs) then lemma7 (remove_op tr (id, (C.Add v))) s1 (remove_op tr (id, (C.Add v)))
+                      else lemma7 (remove_op tr (id, (C.Add v))) (remove_st v s1) (remove_op tr (id, (C.Add v)))
+  |[], (_, (C.Add v))::xs -> ()
+
+val lemma8 : ltr:ae op 
+           -> atr:ae op 
+           -> Lemma (requires (forall e. mem e ltr.l ==> not (member (get_id e) atr.l)) /\
+                             (forall i e. mem e (project i ltr).l ==> not (member (get_id e) (project i atr).l)))
+                   (ensures (forall i e. mem e (union (project i ltr) (project i atr)).l <==>
+                                    mem e (project i (union ltr atr)).l) /\
+                            (forall i. (forall e e1. (mem e (union (project i ltr) (project i atr)).l /\ 
+             mem e1 (union (project i ltr) (project i atr)).l /\ get_id e <> get_id e1 /\ 
+                    (union (project i ltr) (project i atr)).vis e e1) <==>
+            (mem e (project i (union ltr atr)).l /\ mem e1 (project i (union ltr atr)).l /\ get_id e <> get_id e1 /\
+                   (project i (union ltr atr)).vis e e1))))
+
+#set-options "--z3rlimit 10000000"
+let lemma8 ltr atr = ()
+
+val lemma9 : ltr:ae op 
+           -> atr:ae op 
+           -> btr:ae op 
+           -> Lemma (requires (forall e. mem e ltr.l ==> not (member (get_id e) atr.l)) /\
+                             (forall e. mem e atr.l ==> not (member (get_id e) btr.l)) /\
+                             (forall e. mem e ltr.l ==> not (member (get_id e) btr.l))/\
+                             (forall i e. mem e (project i ltr).l ==> not (member (get_id e) (project i atr).l)) /\
+                             (forall i e. mem e (project i atr).l ==> not (member (get_id e) (project i btr).l)) /\
+                             (forall i e. mem e (project i ltr).l ==> not (member (get_id e) (project i btr).l)))
+                   (ensures (forall i. (forall e. mem e (absmerge (project i ltr) (project i atr) (project i btr)).l <==>
+                             mem e (project i (absmerge ltr atr btr)).l)) /\
+             (forall i. (forall e e1. mem e (absmerge (project i ltr) (project i atr) (project i btr)).l /\
+                  mem e1 (absmerge (project i ltr) (project i atr) (project i btr)).l /\ get_id e <> get_id e1 /\
+                              (absmerge (project i ltr) (project i atr) (project i btr)).vis e e1 <==>
+                                mem e (project i (absmerge ltr atr btr)).l /\ mem e1 (project i (absmerge ltr atr btr)).l /\ get_id e <> get_id e1 /\ (project i (absmerge ltr atr btr)).vis e e1)))
+
+#set-options "--z3rlimit 10000000"
+let lemma9 ltr atr btr = ()
+
+val prop_merge1 : ltr:ae op
+                -> l:s
+                -> atr:ae op
+                -> a:s
+                -> btr:ae op
+                -> b:s
+                -> chs:list nat
+                -> Lemma (requires (forall e. mem e ltr.l ==> not (member (get_id e) atr.l)) /\
+                                  (forall e. mem e atr.l ==> not (member (get_id e) btr.l)) /\
+                                  (forall e. mem e ltr.l ==> not (member (get_id e) btr.l)) /\
+                                  (sim ltr l /\ sim (union ltr atr) a /\ sim (union ltr btr) b) /\
+                                  (forall i. mem_key_s i l ==> mem_key_s i a /\ mem_key_s i b) /\
+                                  (forall i. mem i chs ==> mem_key_s i (merge ltr l atr a btr b)))
+                        (ensures (forall i. mem i chs ==> 
+                            (C.sim (project i (absmerge ltr atr btr)) (get_val_s i (merge ltr l atr a btr b)))))
+                (decreases chs)
+
+#set-options "--z3rlimit 10000000"
+let rec prop_merge1 ltr l atr a btr b lst =
+  match lst with
+  |[] -> ()
+  |i::is -> lemma8 ltr atr; lemma8 ltr btr;
+          lemma7 (project i (union ltr atr)) (get_val_s i a) (union (project i ltr) (project i atr));
+          lemma7 (project i (union ltr btr)) (get_val_s i b) (union (project i ltr) (project i btr));
+     C.prop_merge (project i ltr) (get_val_s i l) (project i atr) (get_val_s i a) (project i btr) (get_val_s i b);
+          lemma9 ltr atr btr;
+          lemma7 (absmerge (project i ltr) (project i atr) (project i btr)) 
+                 (get_val_s i (merge ltr l atr a btr b)) (project i (absmerge ltr atr btr));
+          assert (C.sim (project i (absmerge ltr atr btr)) (get_val_s i (merge ltr l atr a btr b)));
+          prop_merge1 ltr l atr a btr b is
+
+val prop_merge21 : ltr:ae op
+               -> l:s
+               -> atr:ae op
+               -> a:s
+               -> btr:ae op
+               -> b:s
+               -> Lemma (requires (forall e. mem e ltr.l ==> not (member (get_id e) atr.l)) /\
+                                 (forall e. mem e atr.l ==> not (member (get_id e) btr.l)) /\
+                                 (forall e. mem e ltr.l ==> not (member (get_id e) btr.l)) /\
+                                 (sim ltr l /\ sim (union ltr atr) a /\ sim (union ltr btr) b))
+             (ensures (forall e. mem e (merge ltr l atr a btr b) ==> mem_key (get_key_s e) (absmerge ltr atr btr).l))
+
+#set-options "--z3rlimit 10000000"
+let prop_merge21 ltr l atr a btr b = 
+  lemma2 (merge ltr l atr a btr b);
+  lemma6 ltr atr; lemma6 ltr btr;
+  lemma61 ltr atr btr
+
+val prop_merge22 : ltr:ae op
+               -> l:s
+               -> atr:ae op
+               -> a:s
+               -> btr:ae op
+               -> b:s
+               -> Lemma (requires (forall e. mem e ltr.l ==> not (member (get_id e) atr.l)) /\
+                                 (forall e. mem e atr.l ==> not (member (get_id e) btr.l)) /\
+                                 (forall e. mem e ltr.l ==> not (member (get_id e) btr.l)) /\
+                                 (sim ltr l /\ sim (union ltr atr) a /\ sim (union ltr btr) b))
+           (ensures (forall e. mem e (absmerge ltr atr btr).l ==> mem_key_s (get_key e) (merge ltr l atr a btr b)))
+
+#set-options "--z3rlimit 10000000"
+let prop_merge22 ltr l atr a btr b = 
+  lemma2 (merge ltr l atr a btr b);
+  lemma6 ltr atr; lemma6 ltr btr;
+  lemma61 ltr atr btr
+
+val prop_merge2 : ltr:ae op
+               -> l:s
+               -> atr:ae op
+               -> a:s
+               -> btr:ae op
+               -> b:s
+               -> Lemma (requires (forall e. mem e ltr.l ==> not (member (get_id e) atr.l)) /\
+                                 (forall e. mem e atr.l ==> not (member (get_id e) btr.l)) /\
+                                 (forall e. mem e ltr.l ==> not (member (get_id e) btr.l)) /\
+                                 (sim ltr l /\ sim (union ltr atr) a /\ sim (union ltr btr) b))
+               (ensures (forall ch. mem_key_s ch (merge ltr l atr a btr b) <==> mem_key ch (absmerge ltr atr btr).l))
+
+#set-options "--z3rlimit 10000000"
+let prop_merge2 ltr l atr a btr b = 
+  prop_merge21 ltr l atr a btr b;
+  prop_merge22 ltr l atr a btr b
+
+val prop_merge31 : ltr:ae op
+                  -> l:s
+                  -> atr:ae op
+                  -> a:s
+                  -> btr:ae op
+                  -> b:s
+                  -> Lemma (requires (forall e. mem e ltr.l ==> not (member (get_id e) atr.l)) /\
+                                    (forall e. mem e atr.l ==> not (member (get_id e) btr.l)) /\
+                                    (forall e. mem e ltr.l ==> not (member (get_id e) btr.l)) /\
+                                    (sim ltr l /\ sim (union ltr atr) a /\ sim (union ltr btr) b) /\
+                       (forall ch. mem_key_s ch (merge ltr l atr a btr b) <==> mem_key ch (absmerge ltr atr btr).l))
+                    (ensures (forall e. mem e (absmerge ltr atr btr).l ==> 
+                             (exists e1. mem e1 (merge ltr l atr a btr b) /\ get_key e = get_key_s e1)))
+
+#set-options "--z3rlimit 10000000"
+let prop_merge31 ltr l atr a btr b = 
+  lemma2 (merge ltr l atr a btr b);
+  lemma6 ltr atr; lemma6 ltr btr;
+  lemma61 ltr atr btr
+
+val prop_merge3 : ltr:ae op
+                  -> l:s
+                  -> atr:ae op
+                  -> a:s
+                  -> btr:ae op
+                  -> b:s
+                  -> Lemma (requires (forall e. mem e ltr.l ==> not (member (get_id e) atr.l)) /\
+                                    (forall e. mem e atr.l ==> not (member (get_id e) btr.l)) /\
+                                    (forall e. mem e ltr.l ==> not (member (get_id e) btr.l)) /\
+                                    (sim ltr l /\ sim (union ltr atr) a /\ sim (union ltr btr) b) /\
+                       (forall ch. mem_key_s ch (merge ltr l atr a btr b) <==> mem_key ch (absmerge ltr atr btr).l) /\
+                       (forall e. mem e (absmerge ltr atr btr).l ==> 
+                                 (exists e1. mem e1 (merge ltr l atr a btr b) /\ get_key e = get_key_s e1)))
+                   (ensures (forall e. mem e (absmerge ltr atr btr).l ==> (exists e1. mem e1 (merge ltr l atr a btr b) /\
+                                  get_key e = get_key_s e1 /\ mem (get_val e) (get_val_s1 e1))))
+
+#set-options "--z3rlimit 10000000"
+let prop_merge3 ltr l atr a btr b = 
+  lemma2 (merge ltr l atr a btr b);
+  lemma6 ltr atr; lemma6 ltr btr;
+  lemma61 ltr atr btr
+  
+val prop_merge : ltr:ae op
+               -> l:s
+               -> atr:ae op
+               -> a:s
+               -> btr:ae op
+               -> b:s
+               -> Lemma (requires (forall e. mem e ltr.l ==> not (member (get_id e) atr.l)) /\
+                                 (forall e. mem e atr.l ==> not (member (get_id e) btr.l)) /\
+                                 (forall e. mem e ltr.l ==> not (member (get_id e) btr.l)) /\
+                                 (sim ltr l /\ sim (union ltr atr) a /\ sim (union ltr btr) b))
+                       (ensures (sim (absmerge ltr atr btr) (merge ltr l atr a btr b)))
+
+#set-options "--z3rlimit 10000000"
+let prop_merge ltr l atr a btr b = 
+  prop_merge2 ltr l atr a btr b;
+  prop_merge31 ltr l atr a btr b;
+  prop_merge3 ltr l atr a btr b;
+  let m = get_lst (merge ltr l atr a btr b) in
+  prop_merge1 ltr l atr a btr b m
+
+instance _ : mrdt s op gmap = {
+  Library.merge = merge;
+  Library.prop_merge = prop_merge;
+  Library.convergence = convergence;
+  Library.sim = sim;
+  Library.prop_oper = prop_oper
+}
